deps/poulet4/lib/P4cub/BigStep/Typing.v
@@ -17,19 +17,19 @@ Import Step P.P4cubNotations
        F.FieldTactics ProperType.
 
 (** Semantic expression typing. *)
-Reserved Notation "'⟦⟦' ers , gm '⟧⟧' ⊨ e ∈ t"
+Reserved Notation "'⟦⟦' dl , gm '⟧⟧' ⊨ e ∈ t"
          (at level 40, e custom p4expr, t custom p4type,
-          gm custom p4env, ers custom p4env).
+          gm custom p4env, dl custom p4env).
 
 (** An expression [e] evaluates in a "well-typed" way.
     Progress & preservation included all in one. *)
 Definition semantic_expr_typing
-           {tags_t : Type} (errs : errors) (Γ : gamma)
+           {tags_t : Type} (D : Delta) (Γ : Gamma)
            (e: E.e tags_t) (t: E.t) : Prop :=
   forall ϵ : epsilon,
-    envs_sound Γ ϵ errs ->
+    envs_sound Γ ϵ D ->
     (exists v : V.v, ⟨ ϵ, e ⟩ ⇓ v) /\
-    (forall v : V.v, ⟨ ϵ, e ⟩ ⇓ v -> ∇ errs ⊢ v ∈ t).
+    (forall v : V.v, ⟨ ϵ, e ⟩ ⇓ v -> ∇ ⊢ v ∈ t).
 
 Notation "'⟦⟦' ers , gm '⟧⟧' ⊨ e ∈ t"
   := (semantic_expr_typing ers gm e t).
@@ -57,23 +57,23 @@ Ltac unfold_sem_typ_expr :=
 (** Typing Derivations. *)
 Section Rules.
   Context {tags_t : Type}.
-  Variable Γ : gamma.
-  Variable errs : errors.
+  Variable Γ : Gamma.
+  Variable D : Delta.
   Variable i : tags_t.
 
   Local Hint Constructors expr_big_step : core.
   Local Hint Constructors type_value : core.
   
   Lemma sem_typ_bool : forall b,
-      ⟦⟦ errs, Γ ⟧⟧ ⊨ BOOL b @ i ∈ Bool.
+      ⟦⟦ D, Γ ⟧⟧ ⊨ BOOL b @ i ∈ Bool.
   Proof.
     intros b; unfold_sem_typ_expr; eauto.
   Qed.
   
   Lemma sem_typ_uop : forall (op : E.uop) (τ τ' : E.t) (e : E.e tags_t),
       uop_type op τ τ' ->
-      ⟦⟦ errs, Γ ⟧⟧ ⊨ e ∈ τ ->
-      ⟦⟦ errs, Γ ⟧⟧ ⊨ UOP op e:τ @ i ∈ τ'.
+      ⟦⟦ D, Γ ⟧⟧ ⊨ e ∈ τ ->
+      ⟦⟦ D, Γ ⟧⟧ ⊨ UOP op e:τ @ i ∈ τ'.
   Proof.
     intros op t t' e Huop He; unfold_sem_typ_expr.
     (* Tedious proof... *)
@@ -83,7 +83,7 @@ Section Rules.
   Local Hint Resolve expr_big_step_progress : core.
   
   Lemma soundness : forall (e : E.e tags_t) τ,
-      ⟦ errs, Γ ⟧ ⊢ e ∈ τ -> ⟦⟦ errs, Γ ⟧⟧ ⊨ e ∈ τ.
+      ⟦ D, Γ ⟧ ⊢ e ∈ τ -> ⟦⟦ D, Γ ⟧⟧ ⊨ e ∈ τ.
   Proof.
     intros e t Ht; intros ϵ H; split; eauto;
       destruct H as (? & ?); eauto.
@@ -92,7 +92,7 @@ Section Rules.
   Local Hint Constructors check_expr : core.
   
   Lemma completeness : forall (e : E.e tags_t) τ,
-      ⟦⟦ errs, Γ ⟧⟧ ⊨ e ∈ τ -> ⟦ errs, Γ ⟧ ⊢ e ∈ τ.
+      ⟦⟦ D, Γ ⟧⟧ ⊨ e ∈ τ -> ⟦ D, Γ ⟧ ⊢ e ∈ τ.
   Proof.
     intro e; induction e using custom_e_ind;
       intros t Hsem; unfold_sem_typ_expr_hyp.
