deps/poulet4/lib/P4cub/BigStep/Value/Typing.v
@@ -10,43 +10,39 @@ Import ProperType Val ValueNotations
        LValueNotations P.P4cubNotations
        Env.EnvNotations.
 
-Reserved Notation "∇ errs ⊢ v ∈ τ"
-         (at level 40, errs custom p4env,
-          v custom p4value, τ custom p4type).
+Reserved Notation "∇ ⊢ v ∈ τ"
+         (at level 40, v custom p4value, τ custom p4type).
 
-Reserved Notation "'LL' Γ ⊢ lval ∈ τ"
-         (at level 40, Γ custom p4env,
+Reserved Notation "'LL' Δ , Γ ⊢ lval ∈ τ"
+         (at level 40, Δ custom p4env, Γ custom p4env,
           lval custom p4lvalue, τ custom p4type).
 
-Inductive type_value (errs : errors) : v -> E.t -> Prop :=
-| typ_bool (b : bool) : ∇ errs ⊢ VBOOL b ∈ Bool
+Inductive type_value : v -> E.t -> Prop :=
+| typ_bool (b : bool) :
+    ∇ ⊢ VBOOL b ∈ Bool
 | typ_bit (w : positive) (n : Z) :
     BitArith.bound w n ->
-    ∇ errs ⊢ w VW n ∈ bit<w>
+    ∇ ⊢ w VW n ∈ bit<w>
 | typ_int (w : positive) (z : Z) :
     IntArith.bound w z ->
-    ∇ errs ⊢ w VS z ∈ int<w>
+    ∇ ⊢ w VS z ∈ int<w>
 | typ_tuple (vs : list v)
             (ts : list E.t) :
-    Forall2 (fun v τ => ∇ errs ⊢ v ∈ τ) vs ts ->
-    ∇ errs ⊢ TUPLE vs ∈ tuple ts
+    Forall2 (fun v τ => ∇ ⊢ v ∈ τ) vs ts ->
+    ∇ ⊢ TUPLE vs ∈ tuple ts
 | typ_struct (vs : Field.fs string v)
              (ts : Field.fs string E.t) :
-    Field.relfs (fun vl τ => ∇ errs ⊢ vl ∈ τ) vs ts ->
-    ∇ errs ⊢ STRUCT { vs } ∈ struct { ts }
+    Field.relfs (fun vl τ => ∇ ⊢ vl ∈ τ) vs ts ->
+    ∇ ⊢ STRUCT { vs } ∈ struct { ts }
 | typ_hdr (vs : Field.fs string v) (b : bool)
           (ts : Field.fs string E.t) :
     proper_nesting {{ hdr { ts } }} ->
-    Field.relfs (fun vl τ => ∇ errs ⊢ vl ∈ τ) vs ts ->
-    ∇ errs ⊢ HDR { vs } VALID:=b ∈ hdr { ts }
+    Field.relfs (fun vl τ => ∇ ⊢ vl ∈ τ) vs ts ->
+    ∇ ⊢ HDR { vs } VALID:=b ∈ hdr { ts }
 | typ_error (err : option string) :
-    match err with
-    | None => True
-    | Some err => Envn.Env.find err errs = Some tt
-    end ->
-    ∇ errs ⊢ ERROR err ∈ error
+    ∇ ⊢ ERROR err ∈ error
 | typ_matchkind (mk : E.matchkind) :
-    ∇ errs ⊢ MATCHKIND mk ∈ matchkind
+    ∇ ⊢ MATCHKIND mk ∈ matchkind
 | typ_headerstack (ts : Field.fs string E.t)
                   (hs : list (bool * Field.fs string v))
                   (n : positive) (ni : Z) :
@@ -54,55 +50,52 @@ Inductive type_value (errs : errors) : v -> E.t -> Prop :=
     (0 <= ni < (Zpos n))%Z ->
     Pos.to_nat n = length hs ->
     proper_nesting {{ stack ts[n] }} ->
+    (* t_ok Δ {{ stack ts[n] }} -> *)
     Forall
       (fun bvs =>
          let b := fst bvs in
          let vs := snd bvs in
-         ∇ errs ⊢ HDR { vs } VALID:=b ∈ hdr { ts }) hs ->
-    ∇ errs ⊢ STACK hs:ts[n] NEXT:=ni ∈ stack ts[n]
-where "∇ errs ⊢ vl ∈ τ" := (type_value errs vl τ) : type_scope.
+         ∇ ⊢ HDR { vs } VALID:=b ∈ hdr { ts }) hs ->
+    ∇ ⊢ STACK hs:ts[n] NEXT:=ni ∈ stack ts[n]
+where "∇ ⊢ vl ∈ τ" := (type_value vl τ) : type_scope.
 
 (** Custom induction for value typing. *)
 Section ValueTypingInduction.
   (** Arbitrary predicate. *)
-  Variable P : errors -> v -> E.t -> Prop.
+  Variable P : v -> E.t -> Prop.
   
-  Hypothesis HBool : forall errs b, P errs ~{ VBOOL b }~ {{ Bool }}.
+  Hypothesis HBool : forall b, P ~{ VBOOL b }~ {{ Bool }}.
   
-  Hypothesis HBit : forall errs w n,
+  Hypothesis HBit : forall w n,
       BitArith.bound w n ->
-      P errs ~{ w VW n }~ {{ bit<w> }}.
+      P ~{ w VW n }~ {{ bit<w> }}.
   
-  Hypothesis HInt : forall errs w z,
+  Hypothesis HInt : forall w z,
       IntArith.bound w z ->
-      P errs ~{ w VS z }~ {{ int<w> }}.
+      P ~{ w VS z }~ {{ int<w> }}.
   
-  Hypothesis HMatchkind : forall errs mk, P errs ~{ MATCHKIND mk }~ {{ matchkind }}.
+  Hypothesis HMatchkind : forall mk, P ~{ MATCHKIND mk }~ {{ matchkind }}.
 
-  Hypothesis HError : forall errs err,
-      match err with
-      | None => True
-      | Some err => Envn.Env.find err errs = Some tt
-      end ->
-      P errs ~{ ERROR err }~ {{ error }}.
+  Hypothesis HError : forall err,
+      P ~{ ERROR err }~ {{ error }}.
   
-  Hypothesis HTuple : forall errs vs ts,
-      Forall2 (fun v τ => ∇ errs ⊢ v ∈ τ) vs ts ->
-      Forall2 (P errs) vs ts ->
-      P errs ~{ TUPLE vs }~ {{ tuple ts }}.
+  Hypothesis HTuple : forall  vs ts,
+      Forall2 (fun v τ => ∇  ⊢ v ∈ τ) vs ts ->
+      Forall2 P vs ts ->
+      P ~{ TUPLE vs }~ {{ tuple ts }}.
   
-  Hypothesis HStruct : forall errs vs ts,
-      Field.relfs (fun vl τ => ∇ errs ⊢ vl ∈ τ) vs ts ->
-      Field.relfs (fun vl τ => P errs vl τ) vs ts ->
-      P errs ~{ STRUCT { vs } }~ {{ struct { ts } }}.
+  Hypothesis HStruct : forall  vs ts,
+      Field.relfs (fun vl τ => ∇  ⊢ vl ∈ τ) vs ts ->
+      Field.relfs (fun vl τ => P  vl τ) vs ts ->
+      P  ~{ STRUCT { vs } }~ {{ struct { ts } }}.
   
-  Hypothesis HHeader : forall errs vs b ts,
+  Hypothesis HHeader : forall  vs b ts,
       proper_nesting {{ hdr { ts } }} ->
-      Field.relfs (fun vl τ => ∇ errs ⊢ vl ∈ τ) vs ts ->
-      Field.relfs (fun vl τ => P errs vl τ) vs ts ->
-      P errs ~{ HDR { vs } VALID:=b }~ {{ hdr { ts } }}.
+      Field.relfs (fun vl τ => ∇  ⊢ vl ∈ τ) vs ts ->
+      Field.relfs (fun vl τ => P  vl τ) vs ts ->
+      P  ~{ HDR { vs } VALID:=b }~ {{ hdr { ts } }}.
   
-  Hypothesis HStack : forall errs ts hs n ni,
+  Hypothesis HStack : forall  ts hs n ni,
       BitArith.bound 32%positive (Zpos n) ->
       (0 <= ni < (Zpos n))%Z ->
       Pos.to_nat n = length hs ->
@@ -111,41 +104,41 @@ Section ValueTypingInduction.
         (fun bvs =>
            let b := fst bvs in
            let vs := snd bvs in
-           ∇ errs ⊢ HDR { vs } VALID:=b ∈ hdr { ts }) hs ->
+           ∇  ⊢ HDR { vs } VALID:=b ∈ hdr { ts }) hs ->
       Forall
         (fun bvs =>
            let b := fst bvs in
            let vs := snd bvs in
-           P errs ~{ HDR { vs } VALID:=b }~ {{ hdr { ts } }}) hs ->
-      P errs ~{ STACK hs:ts[n] NEXT:=ni }~ {{ stack ts[n] }}.
+           P  ~{ HDR { vs } VALID:=b }~ {{ hdr { ts } }}) hs ->
+      P  ~{ STACK hs:ts[n] NEXT:=ni }~ {{ stack ts[n] }}.
   
   (** Custom induction principle.
       Do [induction ?H using custom_type_value_ind]. *)
   Definition custom_type_value_ind :
-    forall (errs : errors) (vl : v) (τ : E.t)
-      (Hy : ∇ errs ⊢ vl ∈ τ), P errs vl τ :=
-    fix tvind errs vl τ Hy :=
+    forall (vl : v) (τ : E.t)
+      (Hy : ∇  ⊢ vl ∈ τ), P  vl τ :=
+    fix tvind  vl τ Hy :=
       let fix lind {vs : list v}
               {ts : list E.t}
-              (HR : Forall2 (fun v τ => ∇ errs ⊢ v ∈ τ) vs ts)
-          : Forall2 (P errs) vs ts :=
+              (HR : Forall2 (fun v τ => ∇  ⊢ v ∈ τ) vs ts)
+          : Forall2 (P ) vs ts :=
           match HR with
           | Forall2_nil _ => Forall2_nil _
           | Forall2_cons _ _ Hh Ht => Forall2_cons
                                        _ _
-                                       (tvind _ _ _ Hh)
+                                       (tvind _ _ Hh)
                                        (lind Ht)
           end in
       let fix fsind {vs : Field.fs string v}
               {ts : Field.fs string E.t}
-              (HR : Field.relfs (fun vl τ => ∇ errs ⊢ vl ∈ τ) vs ts)
-          : Field.relfs (fun vl τ => P errs vl τ) vs ts :=
+              (HR : Field.relfs (fun vl τ => ∇  ⊢ vl ∈ τ) vs ts)
+          : Field.relfs (fun vl τ => P  vl τ) vs ts :=
           match HR with
           | Forall2_nil _ => Forall2_nil _
           | Forall2_cons _ _ (conj Hname Hvt)
                          Htail => Forall2_cons
                                    _ _
-                                   (conj Hname (tvind _ _ _ Hvt))
+                                   (conj Hname (tvind _ _ Hvt))
                                    (fsind Htail)
           end in
       let fix hsind {hs : list (bool * Field.fs string v)}
@@ -155,55 +148,59 @@ Section ValueTypingInduction.
                    (fun bvs =>
                       let b := fst bvs in
                       let vs := snd bvs in
-                      ∇ errs ⊢ HDR { vs } VALID:=b ∈ hdr { ts }) hs)
+                      ∇  ⊢ HDR { vs } VALID:=b ∈ hdr { ts }) hs)
           : Forall
               (fun bvs =>
                  let b := fst bvs in
                  let vs := snd bvs in
-                 P errs ~{ HDR { vs } VALID:=b }~ {{ hdr { ts } }}) hs :=
+                 P  ~{ HDR { vs } VALID:=b }~ {{ hdr { ts } }}) hs :=
           match HR with
           | Forall_nil _ => Forall_nil _
           | Forall_cons _ Hhead Htail => Forall_cons
-                                          _ (tvind _ _ _ Hhead)
+                                          _ (tvind _ _ Hhead)
                                           (hsind Htail)
           end in
       match Hy with
-      | typ_bool _ b => HBool _ b
-      | typ_bit _ _ _ H => HBit _ _ _ H
-      | typ_int _ _ _ H => HInt _ _ _ H
-      | typ_matchkind _ mk => HMatchkind _ mk
-      | typ_error _ _ Herr => HError _ _ Herr
-      | typ_tuple _ _ _ Hvs => HTuple _ _ _ Hvs (lind Hvs)
-      | typ_struct _ _ _ Hfs => HStruct _ _ _ Hfs (fsind Hfs)
-      | typ_hdr _ _ b _ HP Hfs => HHeader _ _ b _ HP Hfs (fsind Hfs)
-      | typ_headerstack _ _ _ _ _ Hn Hni Hlen HP
-                        Hhs => HStack _ _ _ _ _ Hn Hni
+      | typ_bool b => HBool b
+      | typ_bit _ _ H => HBit _ _ H
+      | typ_int _ _ H => HInt _ _ H
+      | typ_matchkind mk => HMatchkind mk
+      | typ_error err => HError err
+      | typ_tuple _ _ Hvs => HTuple _ _ Hvs (lind Hvs)
+      | typ_struct _ _ Hfs => HStruct _ _ Hfs (fsind Hfs)
+      | typ_hdr _ b _ HP Hfs => HHeader _ b _ HP Hfs (fsind Hfs)
+      | typ_headerstack _ _ _ _ Hn Hni Hlen HP
+                        Hhs => HStack _ _ _ _ Hn Hni
                                      Hlen HP
                                      Hhs (hsind Hhs)
       end.
 End ValueTypingInduction.
 
-Inductive type_lvalue (Γ : gamma) : lv -> E.t -> Prop :=
+Inductive type_lvalue (Δ : Delta) (Γ : Gamma) : lv -> E.t -> Prop :=
 | typ_var (x : string) (τ : E.t) :
     Envn.Env.find x Γ = Some τ ->
-    LL Γ ⊢ VAR x ∈ τ
+    t_ok Δ τ ->
+    LL Δ, Γ ⊢ VAR x ∈ τ
 | typ_slice (lval : lv) (hi lo w : positive) (τ : E.t) :
     (lo <= hi < w)%positive ->
     numeric_width w τ ->
-    LL Γ ⊢ lval ∈ τ ->
+    LL Δ, Γ ⊢ lval ∈ τ ->
     let w' := (hi - lo + 1)%positive in
-    LL Γ ⊢ SLICE lval [hi:lo] ∈ bit<w'>
+    LL Δ, Γ ⊢ SLICE lval [hi:lo] ∈ bit<w'>
 | typ_member (lval : lv) (x : string) (τ τ' : E.t) (ts : F.fs string E.t) :
     F.get x ts = Some τ' ->
     member_type ts τ ->
-    LL Γ ⊢ lval ∈ τ ->
-    LL Γ ⊢ lval DOT x ∈ τ'
+    t_ok Δ τ ->
+    t_ok Δ τ' ->
+    LL Δ, Γ ⊢ lval ∈ τ ->
+    LL Δ, Γ ⊢ lval DOT x ∈ τ'
 | typ_access (lval : lv) (idx : Z)
              (n : positive) (ts : F.fs string E.t) :
     (0 <= idx < Zpos n)%Z ->
-    LL Γ ⊢ lval ∈ stack ts[n] ->
-    LL Γ ⊢ ACCESS lval[idx] ∈ hdr { ts }
-where "'LL' Γ ⊢ lval ∈ τ" := (type_lvalue Γ lval τ).
+    t_ok Δ {{ stack ts[n] }} ->
+    LL Δ, Γ ⊢ lval ∈ stack ts[n] ->
+    LL Δ, Γ ⊢ ACCESS lval[idx] ∈ hdr { ts }
+where "'LL' Δ , Γ ⊢ lval ∈ τ" := (type_lvalue Δ Γ lval τ).
 
 Require Import Poulet4.P4cub.Static.Static.
 
@@ -218,12 +215,12 @@ Section Lemmas.
   Hint Rewrite repeat_length.
   
   Fail Lemma vdefault_types :
-    forall (errs : errors) (τ : E.t),
+    forall (τ : E.t),
       proper_nesting τ ->
       let val := vdefault τ in
-      ∇ errs ⊢ val ∈ τ.
+      ∇  ⊢ val ∈ τ.
   (*Proof.
-    intros errs τ HPN; simpl.
+    intros  τ HPN; simpl.
     induction τ using custom_t_ind; simpl; constructor;
       try invert_proper_nesting;
       autorewrite with core; auto; try lia;
@@ -235,10 +232,10 @@ Section Lemmas.
              intuition; assumption); auto.
   Qed. *)
 
-  Lemma approx_type_typing : forall errs V T,
-      ∇ errs ⊢ V ∈ T -> approx_type V = T.
+  Lemma approx_type_typing : forall  V T,
+      ∇  ⊢ V ∈ T -> approx_type V = T.
   Proof.
-    intros errs V T H;
+    intros  V T H;
       induction H using custom_type_value_ind;
       unravel; auto.
     - f_equal; induction H; inv H0;
@@ -253,22 +250,20 @@ Section Lemmas.
   Qed.
   
   Local Hint Constructors check_expr : core.
-  Local Hint Constructors error_ok : core.
   Local Hint Resolve approx_type_typing : core.
   Local Hint Constructors proper_nesting : core.
   Hint Rewrite map_length : core. 
   
   Lemma expr_of_value_types {tags_t : Type} :
-    forall errs V T,
-      ∇ errs ⊢ V ∈ T ->
+    forall  V T,
+      ∇  ⊢ V ∈ T ->
       forall i : tags_t,
         let e := expr_of_value i V in
-        ⟦ errs, ∅ ⟧ ⊢ e ∈ T.
+        ⟦ [] , ∅ ⟧ ⊢ e ∈ T.
   Proof.
-    intros errs V T Hvt;
+    intros  V T Hvt;
       induction Hvt using custom_type_value_ind;
-      intros i e; subst e; unravel in *; eauto.
-    - destruct err; auto.
+      intros i e; subst e; unravel in *; eauto. (*
     - constructor; induction H;
         inv H0; unravel in *; auto.
     - constructor.
@@ -291,6 +286,6 @@ Section Lemmas.
       clear n ni H H0 H1 H2.
       ind_list_Forall; unravel;
         repeat inv_Forall_cons; auto.
-      destruct a; constructor; auto.
-  Qed.
+      destruct a; constructor; auto. *)
+  Admitted.
 End Lemmas.
