deps/poulet4/lib/P4cub/Static/Typing.v
@@ -6,42 +6,41 @@ Require Import Coq.PArith.BinPos Coq.ZArith.BinInt
 (* TODO: type parameters, arguments, ok types. *)
 
 (** Expression typing. *)
-Reserved Notation "⟦ ers , gm ⟧ ⊢ e ∈ t"
+Reserved Notation "⟦ dl , gm ⟧ ⊢ e ∈ t"
          (at level 40, e custom p4expr, t custom p4type,
-          gm custom p4env, ers custom p4env).
+          gm custom p4env, dl custom p4env).
 
 (** Statement typing. *)
-Reserved Notation "⦃ fns , errs , g1 ⦄ ctx ⊢ s ⊣ ⦃ g2 , sg ⦄"
+Reserved Notation "⦃ fns , dl , g1 ⦄ ctx ⊢ s ⊣ ⦃ g2 , sg ⦄"
          (at level 40, s custom p4stmt, ctx custom p4context,
           g2 custom p4env, sg custom p4signal,
-          g1 custom p4env, fns custom p4env, errs custom p4env).
+          g1 custom p4env, fns custom p4env, dl custom p4env).
 
 (** Parser-expression typing. *)
-Reserved Notation "⟅ sts , ers , gm ⟆ ⊢ e"
+Reserved Notation "⟅ sts , dl , gm ⟆ ⊢ e"
          (at level 40, e custom p4prsrexpr,
-          sts custom p4env, ers custom p4env, gm custom p4env).
+          sts custom p4env, dl custom p4env, gm custom p4env).
 
 (** Parser-state-block typing. *)
-Reserved Notation "'⟅⟅' fns , pis , eis , sts , errs , Γ '⟆⟆' ⊢ s"
+Reserved Notation "'⟅⟅' fns , pis , eis , sts , dl , Γ '⟆⟆' ⊢ s"
          (at level 40, s custom p4prsrstateblock,
           fns custom p4env, pis custom p4env,
           eis custom p4env, sts custom p4env,
-          errs custom p4env, Γ custom p4env).
+          dl custom p4env, Γ custom p4env).
 
 (** Control-declaration typing. *)
 Reserved Notation
-         "⦅ ts1 , as1 , fs , ci , ei , errs , g ⦆ ⊢ d ⊣ ⦅ as2 , ts2 ⦆"
+         "⦅ ts1 , as1 , fs , ci , ei , g ⦆ ⊢ d ⊣ ⦅ as2 , ts2 ⦆"
          (at level 60, d custom p4ctrldecl,
           ts1 custom p4env, as1 custom p4env,
           ts2 custom p4env, as2 custom p4env,
           fs custom p4env, ci custom p4env,
-          ei custom p4env, errs custom p4env,
-          g custom p4env).
+          ei custom p4env, g custom p4env).
 
 (** Toplevel-declaration typing. *)
 Reserved Notation
-         "⦗ cs1 , fs1 , pgi1 , ci1 , pi1 , ei1 , ers ⦘ ⊢ d ⊣ ⦗ ei2 , pi2 , ci2 , pgi2 , fs2 , cs2 ⦘"
-         (at level 70, d custom p4topdecl, ers custom p4env,
+         "⦗ cs1 , fs1 , pgi1 , ci1 , pi1 , ei1 ⦘ ⊢ d ⊣ ⦗ ei2 , pi2 , ci2 , pgi2 , fs2 , cs2 ⦘"
+         (at level 70, d custom p4topdecl,
           ei1 custom p4env, pi1 custom p4env,
           ei2 custom p4env, pi2 custom p4env,
           ci1 custom p4env, fs1 custom p4env,
@@ -62,81 +61,85 @@ Import Env.EnvNotations.
 
 (** Expression typing as a relation. *)
 Inductive check_expr
-          {tags_t : Type} (errs : errors) (Γ : gamma)
+          {tags_t : Type} (Δ : Delta) (Γ : Gamma)
   : E.e tags_t -> E.t -> Prop :=
 (* Literals. *)
 | chk_bool (b : bool) (i : tags_t) :
-    ⟦ errs , Γ ⟧ ⊢ BOOL b @ i ∈ Bool
+    ⟦ Δ , Γ ⟧ ⊢ BOOL b @ i ∈ Bool
 | chk_bit (w : positive) (n : Z) (i : tags_t) :
     BitArith.bound w n ->
-    ⟦ errs , Γ ⟧ ⊢ w W n @ i ∈ bit<w>
+    ⟦ Δ , Γ ⟧ ⊢ w W n @ i ∈ bit<w>
 | chk_int (w : positive) (n : Z) (i : tags_t) :
     IntArith.bound w n ->
-    ⟦ errs , Γ ⟧ ⊢ w S n @ i ∈ int<w>
+    ⟦ Δ , Γ ⟧ ⊢ w S n @ i ∈ int<w>
 | chk_var (x : string) (τ : E.t) (i : tags_t) :
     Env.find x Γ = Some τ ->
+    t_ok Δ τ ->
     PT.proper_nesting τ ->
-    ⟦ errs , Γ ⟧ ⊢ Var x:τ @ i ∈ τ
+    ⟦ Δ , Γ ⟧ ⊢ Var x:τ @ i ∈ τ
 | chk_slice (e : E.e tags_t) (τ : E.t)
             (hi lo w : positive) (i : tags_t) :
     (lo <= hi < w)%positive ->
     numeric_width w τ ->
-    ⟦ errs, Γ ⟧ ⊢ e ∈ τ ->
+    ⟦ Δ, Γ ⟧ ⊢ e ∈ τ ->
     let w' := (hi - lo + 1)%positive in
-    ⟦ errs, Γ ⟧ ⊢ Slice e:τ [hi:lo] @ i ∈ bit<w'>
+    ⟦ Δ, Γ ⟧ ⊢ Slice e:τ [hi:lo] @ i ∈ bit<w'>
 | chk_cast (τ τ' : E.t) (e : E.e tags_t) (i : tags_t) :
     proper_cast τ' τ ->
-    ⟦ errs, Γ ⟧ ⊢ e ∈ τ' ->
-    ⟦ errs, Γ ⟧ ⊢ Cast e:τ @ i ∈ τ
+    t_ok Δ τ' ->
+    t_ok Δ τ ->
+    ⟦ Δ, Γ ⟧ ⊢ e ∈ τ' ->
+    ⟦ Δ, Γ ⟧ ⊢ Cast e:τ @ i ∈ τ
 (* Unary operations. *)
 | chk_uop (op : E.uop) (τ τ' : E.t) (e : E.e tags_t) (i : tags_t) :
     uop_type op τ τ' ->
-    ⟦ errs, Γ ⟧ ⊢ e ∈ τ ->
-    ⟦ errs, Γ ⟧ ⊢ UOP op e:τ @ i ∈ τ'
+    ⟦ Δ, Γ ⟧ ⊢ e ∈ τ ->
+    ⟦ Δ, Γ ⟧ ⊢ UOP op e:τ @ i ∈ τ'
 (* Binary Operations. *)
 | chk_bop (op : E.bop) (τ1 τ2 τ : E.t) (e1 e2 : E.e tags_t) (i : tags_t) :
     bop_type op τ1 τ2 τ ->
-    ⟦ errs , Γ ⟧ ⊢ e1 ∈ τ1 ->
-    ⟦ errs , Γ ⟧ ⊢ e2 ∈ τ2 ->
-    ⟦ errs , Γ ⟧ ⊢ BOP e1:τ1 op e2:τ2 @ i ∈ τ
+    ⟦ Δ , Γ ⟧ ⊢ e1 ∈ τ1 ->
+    ⟦ Δ , Γ ⟧ ⊢ e2 ∈ τ2 ->
+    ⟦ Δ , Γ ⟧ ⊢ BOP e1:τ1 op e2:τ2 @ i ∈ τ
 (* Member expressions. *)
 | chk_mem (e : E.e tags_t) (x : string)
           (fs : F.fs string E.t)
           (τ τ' : E.t) (i : tags_t) :
     F.get x fs = Some τ' ->
     member_type fs τ ->
-    ⟦ errs, Γ ⟧ ⊢ e ∈ τ ->
-    ⟦ errs, Γ ⟧ ⊢ Mem e:τ dot x @ i ∈ τ'
+    t_ok Δ τ ->
+    t_ok Δ τ' ->
+    ⟦ Δ, Γ ⟧ ⊢ e ∈ τ ->
+    ⟦ Δ, Γ ⟧ ⊢ Mem e:τ dot x @ i ∈ τ'
 (* Structs. *)
 | chk_tuple (es : list (E.e tags_t)) (i : tags_t)
             (ts : list E.t) :
-    Forall2 (fun e τ => ⟦ errs, Γ ⟧ ⊢ e ∈ τ) es ts ->
-    ⟦ errs, Γ ⟧ ⊢ tup es @ i ∈ tuple ts
+    Forall2 (fun e τ => ⟦ Δ, Γ ⟧ ⊢ e ∈ τ) es ts ->
+    ⟦ Δ, Γ ⟧ ⊢ tup es @ i ∈ tuple ts
 | chk_struct_lit (efs : F.fs string (E.t * E.e tags_t))
                  (tfs : F.fs string E.t) (i : tags_t) :
     F.relfs
       (fun te τ =>
-         (fst te) = τ /\
+         (fst te) = τ /\ t_ok Δ τ /\
          let e := snd te in
-         ⟦ errs , Γ ⟧ ⊢ e ∈ τ) efs tfs ->
-    ⟦ errs , Γ ⟧ ⊢ struct { efs } @ i ∈ struct { tfs }
+         ⟦ Δ , Γ ⟧ ⊢ e ∈ τ) efs tfs ->
+    ⟦ Δ , Γ ⟧ ⊢ struct { efs } @ i ∈ struct { tfs }
 | chk_hdr_lit (efs : F.fs string (E.t * E.e tags_t))
               (tfs : F.fs string E.t)
               (i : tags_t) (b : E.e tags_t) :
     PT.proper_nesting {{ hdr { tfs } }} ->
     F.relfs
       (fun te τ =>
-         (fst te) = τ /\
+         (fst te) = τ /\ t_ok Δ τ /\
          let e := snd te in
-         ⟦ errs , Γ ⟧ ⊢ e ∈ τ) efs tfs ->
-    ⟦ errs, Γ ⟧ ⊢ b ∈ Bool ->
-    ⟦ errs , Γ ⟧ ⊢ hdr { efs } valid := b @ i ∈ hdr { tfs }
+         ⟦ Δ , Γ ⟧ ⊢ e ∈ τ) efs tfs ->
+    ⟦ Δ, Γ ⟧ ⊢ b ∈ Bool ->
+    ⟦ Δ , Γ ⟧ ⊢ hdr { efs } valid := b @ i ∈ hdr { tfs }
   (* Errors and matchkinds. *)
   | chk_error (err : option string) (i : tags_t) :
-      error_ok errs err ->
-      ⟦ errs , Γ ⟧ ⊢ Error err @ i ∈ error
+      ⟦ Δ , Γ ⟧ ⊢ Error err @ i ∈ error
   | chk_matchkind (mkd : E.matchkind) (i : tags_t) :
-      ⟦ errs , Γ ⟧ ⊢ Matchkind mkd @ i ∈ matchkind
+      ⟦ Δ , Γ ⟧ ⊢ Matchkind mkd @ i ∈ matchkind
   (* Header stacks. *)
   | chk_stack (ts : F.fs string E.t)
               (hs : list (E.e tags_t))
@@ -145,13 +148,15 @@ Inductive check_expr
       (0 <= ni < (Zpos n))%Z ->
       Pos.to_nat n = length hs ->
       PT.proper_nesting {{ stack ts[n] }} ->
-      Forall (fun e => ⟦ errs, Γ ⟧ ⊢ e ∈ hdr { ts }) hs ->
-      ⟦ errs, Γ ⟧ ⊢ Stack hs:ts[n] nextIndex:=ni @ i ∈ stack ts[n]
+      t_ok Δ {{ stack ts[n] }} ->
+      Forall (fun e => ⟦ Δ, Γ ⟧ ⊢ e ∈ hdr { ts }) hs ->
+      ⟦ Δ, Γ ⟧ ⊢ Stack hs:ts[n] nextIndex:=ni @ i ∈ stack ts[n]
   | chk_access (e : E.e tags_t) (idx : Z) (i : tags_t)
                (ts : F.fs string E.t) (n : positive) :
       (0 <= idx < (Zpos n))%Z ->
-      ⟦ errs, Γ ⟧ ⊢ e ∈ stack ts[n] ->
-      ⟦ errs, Γ ⟧ ⊢ Access e[idx] @ i ∈ hdr { ts }
+      t_ok Δ {{ stack ts[n] }} ->
+      ⟦ Δ, Γ ⟧ ⊢ e ∈ stack ts[n] ->
+      ⟦ Δ, Γ ⟧ ⊢ Access e[idx] @ i ∈ hdr { ts }
 where "⟦ ers ',' gm ⟧ ⊢ e ∈ ty"
         := (check_expr ers gm e ty) : type_scope.
 (**[]*)
@@ -178,73 +183,77 @@ Inductive check_pat : PR.pat -> E.t -> Prop :=
                            
 (** Parser-expression typing. *)
 Inductive check_prsrexpr {tags_t : Type}
-          (sts : user_states) (errs : errors) (Γ : gamma)
+          (sts : user_states) (Δ : Delta) (Γ : Gamma)
   : PR.e tags_t -> Prop :=
 | chk_goto (st : PR.state) (i : tags_t) :
     valid_state sts st ->
-    ⟅ sts, errs, Γ ⟆ ⊢ goto st @ i
+    ⟅ sts, Δ, Γ ⟆ ⊢ goto st @ i
 | chk_select (e : E.e tags_t) (def : PR.e tags_t)
              (cases : F.fs PR.pat (PR.e tags_t))
              (i : tags_t) (τ : E.t) :
-    ⟦ errs, Γ ⟧ ⊢ e ∈ τ ->
-    ⟅ sts, errs, Γ ⟆ ⊢ def ->
+    ⟦ Δ, Γ ⟧ ⊢ e ∈ τ ->
+    ⟅ sts, Δ, Γ ⟆ ⊢ def ->
                  Forall
                    (fun pe =>
                       let p := fst pe in
                       let e := snd pe in
-                      check_pat p τ /\ ⟅ sts, errs, Γ ⟆ ⊢ e) cases ->
-                 ⟅ sts, errs, Γ ⟆ ⊢ select e { cases } default:=def @ i
+                      check_pat p τ /\ ⟅ sts, Δ, Γ ⟆ ⊢ e) cases ->
+                 ⟅ sts, Δ, Γ ⟆ ⊢ select e { cases } default:=def @ i
 where "⟅ sts , ers , gm ⟆ ⊢ e"
         := (check_prsrexpr sts ers gm e).
 (**[]*)
   
 (** Statement typing. *)
 Inductive check_stmt
-          {tags_t : Type} (fns : fenv) (errs : errors) (Γ : gamma)
-  : ctx -> ST.s tags_t -> gamma -> signal -> Prop :=
+          {tags_t : Type} (fns : fenv) (Δ : Delta) (Γ : Gamma)
+  : ctx -> ST.s tags_t -> Gamma -> signal -> Prop :=
 | chk_skip (i : tags_t) (con : ctx) :
-    ⦃ fns, errs, Γ ⦄ con ⊢ skip @ i ⊣ ⦃ Γ, C ⦄
-| chk_seq_cont (s1 s2 : ST.s tags_t) (Γ' Γ'' : gamma)
+    ⦃ fns, Δ, Γ ⦄ con ⊢ skip @ i ⊣ ⦃ Γ, C ⦄
+| chk_seq_cont (s1 s2 : ST.s tags_t) (Γ' Γ'' : Gamma)
                (i : tags_t) (sig : signal) (con : ctx) :
-    ⦃ fns, errs, Γ  ⦄ con ⊢ s1 ⊣ ⦃ Γ', C ⦄ ->
-    ⦃ fns, errs, Γ' ⦄ con ⊢ s2 ⊣ ⦃ Γ'', sig ⦄ ->
-    ⦃ fns, errs, Γ  ⦄ con ⊢ s1 ; s2 @ i ⊣ ⦃ Γ'', sig ⦄
-| chk_block (s : ST.s tags_t) (Γ' : gamma) (sig : signal) (con : ctx) :
-    ⦃ fns, errs, Γ ⦄ con ⊢ s ⊣ ⦃ Γ', sig ⦄ ->
-    ⦃ fns, errs, Γ ⦄ con ⊢ b{ s }b ⊣ ⦃ Γ, C ⦄
+    ⦃ fns, Δ, Γ  ⦄ con ⊢ s1 ⊣ ⦃ Γ', C ⦄ ->
+    ⦃ fns, Δ, Γ' ⦄ con ⊢ s2 ⊣ ⦃ Γ'', sig ⦄ ->
+    ⦃ fns, Δ, Γ  ⦄ con ⊢ s1 ; s2 @ i ⊣ ⦃ Γ'', sig ⦄
+| chk_block (s : ST.s tags_t) (Γ' : Gamma) (sig : signal) (con : ctx) :
+    ⦃ fns, Δ, Γ ⦄ con ⊢ s ⊣ ⦃ Γ', sig ⦄ ->
+    ⦃ fns, Δ, Γ ⦄ con ⊢ b{ s }b ⊣ ⦃ Γ, C ⦄
 | chk_vardecl (τ : E.t) (x : string) (i : tags_t) (con : ctx) :
-    ⦃ fns, errs, Γ ⦄ con ⊢ var x:τ @ i ⊣ ⦃ x ↦ τ ;; Γ, C ⦄
+    t_ok Δ τ ->
+    ⦃ fns, Δ, Γ ⦄ con ⊢ var x:τ @ i ⊣ ⦃ x ↦ τ ;; Γ, C ⦄
 | chk_assign (τ : E.t) (e1 e2 : E.e tags_t) (i : tags_t) (con : ctx) :
+    t_ok Δ τ ->
     lvalue_ok e1 ->
-    ⟦ errs, Γ ⟧ ⊢ e1 ∈ τ ->
-    ⟦ errs, Γ ⟧ ⊢ e2 ∈ τ ->
-    ⦃ fns, errs, Γ ⦄ con ⊢ asgn e1 := e2 : τ @ i ⊣ ⦃ Γ, C ⦄
+    ⟦ Δ, Γ ⟧ ⊢ e1 ∈ τ ->
+    ⟦ Δ, Γ ⟧ ⊢ e2 ∈ τ ->
+    ⦃ fns, Δ, Γ ⦄ con ⊢ asgn e1 := e2 : τ @ i ⊣ ⦃ Γ, C ⦄
 | chk_cond (guard : E.e tags_t) (tru fls : ST.s tags_t)
-           (Γ1 Γ2 : gamma) (i : tags_t) (sgt sgf sg : signal) (con : ctx) :
+           (Γ1 Γ2 : Gamma) (i : tags_t) (sgt sgf sg : signal) (con : ctx) :
     lub sgt sgf = sg ->
-    ⟦ errs, Γ ⟧ ⊢ guard ∈ Bool ->
-    ⦃ fns, errs, Γ ⦄ con ⊢ tru ⊣ ⦃ Γ1, sgt ⦄ ->
-    ⦃ fns, errs, Γ ⦄ con ⊢ fls ⊣ ⦃ Γ2, sgf ⦄ ->
-    ⦃ fns, errs, Γ ⦄
+    ⟦ Δ, Γ ⟧ ⊢ guard ∈ Bool ->
+    ⦃ fns, Δ, Γ ⦄ con ⊢ tru ⊣ ⦃ Γ1, sgt ⦄ ->
+    ⦃ fns, Δ, Γ ⦄ con ⊢ fls ⊣ ⦃ Γ2, sgf ⦄ ->
+    ⦃ fns, Δ, Γ ⦄
       con ⊢ if guard:Bool then tru else fls @ i ⊣ ⦃ Γ, sg ⦄
 | chk_return_void (i : tags_t) (con : ctx) :
     return_void_ok con ->
-    ⦃ fns, errs, Γ ⦄ con ⊢ returns @ i ⊣ ⦃ Γ, R ⦄
+    ⦃ fns, Δ, Γ ⦄ con ⊢ returns @ i ⊣ ⦃ Γ, R ⦄
 | chk_return_fruit (τ : E.t) (e : E.e tags_t) (i : tags_t) :
-    ⟦ errs, Γ ⟧ ⊢ e ∈ τ ->
-    ⦃ fns, errs, Γ ⦄ Function τ ⊢ return e:τ @ i ⊣ ⦃ Γ, R ⦄
+    t_ok Δ τ ->
+    ⟦ Δ, Γ ⟧ ⊢ e ∈ τ ->
+    ⦃ fns, Δ, Γ ⦄ Function τ ⊢ return e:τ @ i ⊣ ⦃ Γ, R ⦄
 | chk_exit (i : tags_t) (con : ctx) :
     exit_ctx_ok con ->
-    ⦃ fns, errs, Γ ⦄ con ⊢ exit @ i ⊣ ⦃ Γ, R ⦄
+    ⦃ fns, Δ, Γ ⦄ con ⊢ exit @ i ⊣ ⦃ Γ, R ⦄
 | chk_void_call (params : E.params)
+                (ts : list E.t)
                 (args : E.args tags_t)
                 (f : string) (i : tags_t) (con : ctx) :
     Env.find f fns = Some (P.Arrow params None) ->
     F.relfs
       (P.rel_paramarg_same
-         (fun '(t,e) τ => τ = t /\ ⟦ errs, Γ ⟧ ⊢ e ∈ τ))
+         (fun '(t,e) τ => τ = t /\ ⟦ Δ, Γ ⟧ ⊢ e ∈ τ))
       args params ->
-    ⦃ fns, errs, Γ ⦄ con ⊢ call f <[]> (args) @ i ⊣ ⦃ Γ, C ⦄
+    ⦃ fns, Δ, Γ ⦄ con ⊢ call f<ts>(args) @ i ⊣ ⦃ Γ, C ⦄
 | chk_act_call (params : E.params)
                (args : E.args tags_t)
                (a : string) (i : tags_t)
@@ -253,39 +262,42 @@ Inductive check_stmt
     Env.find a aa = Some params ->
     F.relfs
       (P.rel_paramarg
-         (fun '(t,e) τ => τ = t /\ ⟦ errs, Γ ⟧ ⊢ e ∈ τ)
-         (fun '(t,e) τ => τ = t /\ ⟦ errs, Γ ⟧ ⊢ e ∈ τ /\ lvalue_ok e))
+         (fun '(t,e) τ => τ = t /\ ⟦ Δ, Γ ⟧ ⊢ e ∈ τ)
+         (fun '(t,e) τ => τ = t /\ ⟦ Δ, Γ ⟧ ⊢ e ∈ τ /\ lvalue_ok e))
       args params ->
-    ⦃ fns, errs, Γ ⦄ con ⊢ calling a with args @ i ⊣ ⦃ Γ, C ⦄
+    ⦃ fns, Δ, Γ ⦄ con ⊢ calling a with args @ i ⊣ ⦃ Γ, C ⦄
 | chk_fun_call (τ : E.t) (e : E.e tags_t)
                (params : E.params)
+               (ts : list E.t)
                (args : E.args tags_t)
                (f : string) (i : tags_t) (con : ctx) :
+    t_ok Δ τ ->
     Env.find f fns = Some (P.Arrow params (Some τ)) ->
     F.relfs
       (P.rel_paramarg
-         (fun '(t,e) τ => τ = t /\ ⟦ errs, Γ ⟧ ⊢ e ∈ τ)
-         (fun '(t,e) τ => τ = t /\ ⟦ errs, Γ ⟧ ⊢ e ∈ τ /\ lvalue_ok e))
+         (fun '(t,e) τ => τ = t /\ ⟦ Δ, Γ ⟧ ⊢ e ∈ τ)
+         (fun '(t,e) τ => τ = t /\ ⟦ Δ, Γ ⟧ ⊢ e ∈ τ /\ lvalue_ok e))
       args params ->
-    ⟦ errs, Γ ⟧ ⊢ e ∈ τ ->
-    ⦃ fns, errs, Γ ⦄
-      con ⊢ let e : τ := call f <[]> (args) @ i ⊣ ⦃ Γ, C ⦄
+    ⟦ Δ, Γ ⟧ ⊢ e ∈ τ ->
+    ⦃ fns, Δ, Γ ⦄
+      con ⊢ let e : τ := call f<ts>(args) @ i ⊣ ⦃ Γ, C ⦄
 | chk_apply (eargs : F.fs string string) (args : E.args tags_t) (x : string)
             (i : tags_t) (eps : F.fs string string) (params : E.params)
             (tbls : tblenv) (aa : aenv) (cis : cienv) (eis : eienv) :
     Env.find x cis = Some (eps,params) ->
     F.relfs
       (P.rel_paramarg
-         (fun '(t,e) τ => τ = t /\ ⟦ errs, Γ ⟧ ⊢ e ∈ τ)
-         (fun '(t,e) τ => τ = t /\ ⟦ errs, Γ ⟧ ⊢ e ∈ τ /\ lvalue_ok e))
+         (fun '(t,e) τ => τ = t /\ ⟦ Δ, Γ ⟧ ⊢ e ∈ τ)
+         (fun '(t,e) τ => τ = t /\ ⟦ Δ, Γ ⟧ ⊢ e ∈ τ /\ lvalue_ok e))
       args params ->
-    ⦃ fns, errs, Γ ⦄ ApplyBlock tbls aa cis eis
+    ⦃ fns, Δ, Γ ⦄ ApplyBlock tbls aa cis eis
                      ⊢ apply x with eargs & args @ i ⊣ ⦃ Γ, C ⦄
 | chk_invoke (tbl : string) (i : tags_t) (tbls : tblenv)
              (aa : aenv) (cis : cienv) (eis : eienv) :
-    Env.find tbl tbls = Some tt ->
-    ⦃ fns, errs, Γ ⦄ ApplyBlock tbls aa cis eis ⊢ invoke tbl @ i ⊣ ⦃ Γ, C ⦄
+    In tbl tbls ->
+    ⦃ fns, Δ, Γ ⦄ ApplyBlock tbls aa cis eis ⊢ invoke tbl @ i ⊣ ⦃ Γ, C ⦄
 | chk_extern_call_void (e : string) (f : string)
+                       (ts : list E.t)
                        (args : E.args tags_t) (i : tags_t) (con : ctx)
                        (eis : eienv) (params : E.params)
                        (mhds : F.fs string E.arrowT) :
@@ -294,12 +306,13 @@ Inductive check_stmt
     extern_call_ok eis con ->
     F.relfs
       (P.rel_paramarg
-         (fun '(t,e) τ => τ = t /\ ⟦ errs, Γ ⟧ ⊢ e ∈ τ)
-         (fun '(t,e) τ => τ = t /\ ⟦ errs, Γ ⟧ ⊢ e ∈ τ /\ lvalue_ok e))
+         (fun '(t,e) τ => τ = t /\ ⟦ Δ, Γ ⟧ ⊢ e ∈ τ)
+         (fun '(t,e) τ => τ = t /\ ⟦ Δ, Γ ⟧ ⊢ e ∈ τ /\ lvalue_ok e))
       args params ->
-    ⦃ fns, errs, Γ ⦄
-      con ⊢ extern e calls f <[]> (args) gives None @ i ⊣ ⦃ Γ, C ⦄
+    ⦃ fns, Δ, Γ ⦄
+      con ⊢ extern e calls f<ts>(args) gives None @ i ⊣ ⦃ Γ, C ⦄
 | chk_extern_call_fruit (extrn : string) (f : string)
+                        (ts : list E.t)
                         (args : E.args tags_t) (e : E.e tags_t)
                         (i : tags_t) (con : ctx) (eis : eienv)
                         (params: E.params) (τ : E.t)
@@ -309,12 +322,12 @@ Inductive check_stmt
      extern_call_ok eis con ->
      F.relfs
        (P.rel_paramarg
-          (fun '(t,e) τ => τ = t /\ ⟦ errs, Γ ⟧ ⊢ e ∈ τ)
-          (fun '(t,e) τ => τ = t /\ ⟦ errs, Γ ⟧ ⊢ e ∈ τ /\ lvalue_ok e))
+          (fun '(t,e) τ => τ = t /\ ⟦ Δ, Γ ⟧ ⊢ e ∈ τ)
+          (fun '(t,e) τ => τ = t /\ ⟦ Δ, Γ ⟧ ⊢ e ∈ τ /\ lvalue_ok e))
        args params ->
      let result := Some (τ,e) in
-     (⦃ fns, errs, Γ ⦄
-       con ⊢ extern extrn calls f <[]> (args) gives result @ i ⊣ ⦃ Γ, C ⦄))
+     (⦃ fns, Δ, Γ ⦄
+        con ⊢ extern extrn calls f<ts>(args) gives result @ i ⊣ ⦃ Γ, C ⦄))
 where "⦃ fe , ers , g1 ⦄ con ⊢ s ⊣ ⦃ g2 , sg ⦄"
         := (check_stmt fe ers g1 con s g2 sg).
 (**[]*)
@@ -322,52 +335,51 @@ where "⦃ fe , ers , g1 ⦄ con ⊢ s ⊣ ⦃ g2 , sg ⦄"
 (** Parser State typing. *)
 Inductive check_parser_state
           {tags_t : Type} (fns : fenv) (pis : pienv) (eis : eienv)
-          (sts : user_states) (errs : errors) (Γ : gamma)
+          (sts : user_states) (Δ : Delta) (Γ : Gamma)
   : PR.state_block tags_t -> Prop :=
 | chk_state (s : ST.s tags_t) (e : PR.e tags_t)
-            (Γ' : gamma) (sg : signal) :
-    ⦃ fns, errs, Γ ⦄ Parser pis eis ⊢ s ⊣ ⦃ Γ' , sg ⦄ ->
-    ⟅ sts, errs, Γ' ⟆ ⊢ e ->
-                 ⟅⟅ fns, pis, eis, sts, errs, Γ ⟆⟆ ⊢ state { s } transition e
-where "'⟅⟅' fns , pis , eis , sts , errs , Γ '⟆⟆' ⊢ s"
-        := (check_parser_state fns pis eis sts errs Γ s).
+            (Γ' : Gamma) (sg : signal) :
+    ⦃ fns, Δ, Γ ⦄ Parser pis eis ⊢ s ⊣ ⦃ Γ' , sg ⦄ ->
+    ⟅ sts, Δ, Γ' ⟆ ⊢ e ->
+                 ⟅⟅ fns, pis, eis, sts, Δ, Γ ⟆⟆ ⊢ state { s } transition e
+where "'⟅⟅' fns , pis , eis , sts , Δ , Γ '⟆⟆' ⊢ s"
+        := (check_parser_state fns pis eis sts Δ Γ s).
 (**[]*)
 
 (** Control declaration typing. *)
 Inductive check_ctrldecl {tags_t : Type}
           (tbls : tblenv) (acts : aenv) (fns : fenv)
-          (cis : cienv) (eis : eienv)
-          (errs : errors) (Γ : gamma)
+          (cis : cienv) (eis : eienv) (Γ : Gamma)
   : CD.d tags_t -> aenv -> tblenv -> Prop :=
 | chk_action (a : string)
              (signature : E.params)
              (body : ST.s tags_t) (i : tags_t)
-             (Γ' Γ'' : gamma) (sg : signal) :
+             (Γ' Γ'' : Gamma) (sg : signal) :
     bind_all signature Γ = Γ' ->
-    ⦃ fns, errs, Γ' ⦄ Action acts eis ⊢ body ⊣ ⦃ Γ'', sg ⦄ ->
-    ⦅ tbls, acts, fns, cis, eis, errs, Γ ⦆
+    ⦃ fns, [], Γ' ⦄ Action acts eis ⊢ body ⊣ ⦃ Γ'', sg ⦄ ->
+    ⦅ tbls, acts, fns, cis, eis, Γ ⦆
       ⊢ action a ( signature ) { body } @ i
       ⊣ ⦅ a ↦ signature ;; acts, tbls ⦆
 | chk_table (t : string)
             (kys : list (E.t * E.e tags_t * E.matchkind))
             (actns : list string) (i : tags_t) :
     (* Keys type. *)
-    Forall (fun '(τ,e,_) => ⟦ errs, Γ ⟧ ⊢ e ∈ τ) kys ->
+    Forall (fun '(τ,e,_) => ⟦ [], Γ ⟧ ⊢ e ∈ τ) kys ->
     (* Actions available *)
     Forall (fun a => exists pms, Env.find a acts = Some pms) actns ->
-    ⦅ tbls, acts, fns, cis, eis, errs, Γ ⦆
-      ⊢ table t key:=kys actions:=actns @ i ⊣ ⦅ acts, t ↦ tt;; tbls ⦆
+    ⦅ tbls, acts, fns, cis, eis, Γ ⦆
+      ⊢ table t key:=kys actions:=actns @ i ⊣ ⦅ acts, (t :: tbls) ⦆
 | chk_ctrldecl_seq (d1 d2 : CD.d tags_t) (i : tags_t)
                    (acts' acts'' : aenv) (tbls' tbls'' : tblenv) :
-    ⦅ tbls, acts, fns, cis, eis, errs, Γ ⦆
+    ⦅ tbls, acts, fns, cis, eis, Γ ⦆
       ⊢ d1 ⊣ ⦅ acts', tbls'  ⦆ ->
-    ⦅ tbls', acts', fns, cis, eis, errs, Γ ⦆
+    ⦅ tbls', acts', fns, cis, eis, Γ ⦆
       ⊢ d2 ⊣ ⦅ acts'', tbls'' ⦆ ->
-    ⦅ tbls, acts, fns, cis, eis, errs, Γ  ⦆
+    ⦅ tbls, acts, fns, cis, eis, Γ  ⦆
       ⊢ d1 ;c; d2 @ i ⊣ ⦅ acts'', tbls'' ⦆
 where
-"⦅ ts1 , as1 , fs , ci1 , ei1 , errs , g1 ⦆ ⊢ d ⊣ ⦅ as2 , ts2 ⦆"
-  := (check_ctrldecl ts1 as1 fs ci1 ei1 errs g1 d as2 ts2).
+"⦅ ts1 , as1 , fs , ci1 , ei1 , g1 ⦆ ⊢ d ⊣ ⦅ as2 , ts2 ⦆"
+  := (check_ctrldecl ts1 as1 fs ci1 ei1 g1 d as2 ts2).
 (**[]*)
 
 (** Top-level declaration typing. *)
@@ -375,9 +387,9 @@ where
 Inductive check_topdecl
           {tags_t : Type} (cs : cenv) (fns : fenv)
           (pgis : pkgienv) (cis : cienv) (pis : pienv) (eis : eienv)
-          (errs : errors)
   : TD.d tags_t -> eienv -> pienv -> cienv -> pkgienv -> fenv -> cenv -> Prop :=
 | chk_instantiate_control (c x : string)
+                          (ts : list E.t)
                           (cparams : E.constructor_params)
                           (cargs : E.constructor_args tags_t) (i : tags_t)
                           (extparams : F.fs string string) (params : E.params) :
@@ -386,17 +398,18 @@ Inductive check_topdecl
       (fun carg cparam =>
          match carg, cparam with
          | E.CAExpr e, {{{ VType τ }}}
-           => ⟦ errs , ∅ ⟧ ⊢ e ∈ τ
+           => ⟦ [] , ∅ ⟧ ⊢ e ∈ τ
          | E.CAName ctrl, {{{ ControlType cps eps ps }}}
            => Env.find ctrl cs = Some {{{ ControlType cps eps ps }}}
          (*| E.CAName extrn, {{{ Extern cps { mthds } }}}
            => Env.find extrn cs = Some {{{ Extern cps { mthds } }}}*)
          | _, _ => False
          end) cargs cparams ->
-    ⦗ cs, fns, pgis, cis, pis, eis, errs⦘
-      ⊢ Instance x of c < [] > (cargs) @ i
+    ⦗ cs, fns, pgis, cis, pis, eis ⦘
+      ⊢ Instance x of c<ts>(cargs) @ i
       ⊣ ⦗ eis, pis, x ↦ (extparams,params) ;; cis, pgis, fns, cs ⦘
 | chk_instantiate_parser (p x : string)
+                         (ts : list E.t)
                          (cparams : E.constructor_params)
                          (cargs : E.constructor_args tags_t) (i : tags_t)
                          (extparams : F.fs string string)
@@ -406,15 +419,15 @@ Inductive check_topdecl
       (fun carg cparam =>
          match carg, cparam with
          | E.CAExpr e, {{{ VType τ }}}
-           => ⟦ errs , ∅ ⟧ ⊢ e ∈ τ
+           => ⟦ [] , ∅ ⟧ ⊢ e ∈ τ
          | E.CAName prsr, {{{ ParserType cps eps ps }}}
            => Env.find prsr cs = Some {{{ ParserType cps eps ps }}}
          (*| E.CAName extrn, {{{ Extern cps { mthds } }}}
            => Env.find extrn cs = Some {{{ Extern cps { mthds } }}}*)
          | _, _ => False
          end) cargs cparams ->
-    ⦗ cs, fns, pgis, cis, pis, eis, errs ⦘
-      ⊢ Instance x of p <[]> (cargs) @ i
+    ⦗ cs, fns, pgis, cis, pis, eis ⦘
+      ⊢ Instance x of p<ts>(cargs) @ i
       ⊣ ⦗ eis, x ↦ (extparams,params) ;; pis, cis, pgis, fns, cs ⦘
 (*| chk_instantiate_extern (e x : string)
                          (cparams : E.constructor_params)
@@ -425,14 +438,15 @@ Inductive check_topdecl
       (fun carg cparam =>
          match carg, cparam with
          | E.CAExpr e, {{{ VType τ }}}
-           => ⟦ errs , ∅ ⟧ ⊢ e ∈ τ
+           => ⟦ \Delta , ∅ ⟧ ⊢ e ∈ τ
          | E.CAName extrn, {{{ Extern cps { mthds } }}}
            => Env.find extrn cs = Some {{{ Extern cps { mthds } }}}
          | _, _ => False
          end) cargs cparams ->
-    ⦗ cs, fns, pgis, cis, pis, eis, errs ⦘
+    ⦗ cs, fns, pgis, cis, pis, eis, \Delta ⦘
       ⊢ Instance x of e(cargs) @ i ⊣ ⦗ x ↦ mthds ;; eis, pis, cis, pgis, fns, cs ⦘ *)
 | chk_instantiate_package (pkg x : string)
+                          (ts : list E.t)
                           (cparams : E.constructor_params)
                           (cargs : E.constructor_args tags_t)
                           (i : tags_t) :
@@ -441,7 +455,7 @@ Inductive check_topdecl
       (fun carg cparam =>
          match carg, cparam with
          | E.CAExpr e, {{{ VType τ }}}
-           => ⟦ errs , ∅ ⟧ ⊢ e ∈ τ
+           => ⟦ [] , ∅ ⟧ ⊢ e ∈ τ
          | E.CAName ctrl, {{{ ControlType cps eps ps }}}
            => Env.find ctrl cs = Some {{{ ControlType cps eps ps }}}
          | E.CAName prsr, {{{ ParserType cps eps ps }}}
@@ -451,25 +465,26 @@ Inductive check_topdecl
          | _, _ => False
          end)
       cargs cparams ->
-    ⦗ cs, fns, pgis, cis, pis, eis, errs ⦘
-      ⊢ Instance x of pkg <[]> (cargs) @ i ⊣ ⦗ eis, pis, cis, x ↦ tt ;; pgis, fns, cs ⦘
+    ⦗ cs, fns, pgis, cis, pis, eis ⦘
+      (* TODO: correctly update package instance env *)
+      ⊢ Instance x of pkg<ts>(cargs) @ i ⊣ ⦗ eis, pis, cis, (*x ↦ tt ;;*) pgis, fns, cs ⦘
 | chk_control (c : string) (cparams : E.constructor_params)
               (extparams : F.fs string string)
               (params : E.params) (body : CD.d tags_t)
               (apply_blk : ST.s tags_t) (i : tags_t)
-              (Γ' Γ'' Γ''' : gamma) (sg : signal)
+              (Γ' Γ'' Γ''' : Gamma) (sg : signal)
               (cis' : cienv) (eis' : eienv)
               (tbls : tblenv) (acts : aenv) :
     cbind_all cparams (!{∅}!,pgis,cis,pis,eis) = (Γ',pgis,cis',pis,eis') ->
     (* Control declarations. *)
-    ⦅ ∅, ∅, fns, cis', eis', errs, Γ' ⦆
+    ⦅ [], ∅, fns, cis', eis', Γ' ⦆
       ⊢ body ⊣ ⦅ acts, tbls ⦆ ->
     bind_all params Γ' = Γ'' ->
     (* Apply block. *)
-    ⦃ fns, errs, Γ'' ⦄
+    ⦃ fns, [], Γ'' ⦄
       ApplyBlock tbls acts cis eis ⊢ apply_blk ⊣ ⦃ Γ''', sg ⦄ ->
     let ctor := E.CTControl cparams extparams params in
-    ⦗ cs, fns, pgis, cis, pis, eis, errs ⦘
+    ⦗ cs, fns, pgis, cis, pis, eis ⦘
       ⊢ control c (cparams)(extparams)(params) apply { apply_blk } where { body } @ i
         ⊣ ⦗ eis, pis, cis, pgis, fns, c ↦ ctor;; cs ⦘
 | chk_parser (p : string)
@@ -478,59 +493,63 @@ Inductive check_topdecl
              (params : E.params) (start_state : PR.state_block tags_t)
              (states : F.fs string (PR.state_block tags_t)) (i : tags_t)
              (pis' : pienv) (eis' : eienv)
-             (Γ' Γ'' : gamma) :
+             (Γ' Γ'' : Gamma) :
     let sts := F.fold
-                 (fun st _ acc => !{ st ↦ tt;; acc }!) states !{ ∅ }! in
-    cbind_all cparams (!{∅}!,pgis,cis,pis,eis) = (Γ',pgis,cis,pis',eis') ->
+                 (fun st _ acc => st :: acc) states [] in
+    cbind_all cparams ([],pgis,cis,pis,eis) = (Γ',pgis,cis,pis',eis') ->
     bind_all params Γ' = Γ'' ->
-    ⟅⟅ fns, pis', eis', sts, errs, Γ'' ⟆⟆ ⊢ start_state ->
+    ⟅⟅ fns, pis', eis', sts, [], Γ'' ⟆⟆ ⊢ start_state ->
     F.predfs_data
-      (fun pst => ⟅⟅ fns, pis', eis', sts, errs, Γ'' ⟆⟆ ⊢ pst) states ->
+      (fun pst => ⟅⟅ fns, pis', eis', sts, [], Γ'' ⟆⟆ ⊢ pst) states ->
     let prsr := E.CTParser cparams extparams params in
-    ⦗ cs, fns, pgis, cis, pis, eis, errs ⦘
+    ⦗ cs, fns, pgis, cis, pis, eis ⦘
       ⊢ parser p (cparams)(extparams)(params) start:= start_state { states } @ i
       ⊣ ⦗ eis, pis, cis, pgis, fns, p ↦ prsr;; cs ⦘
 (*| chk_extern (e : string)
              (cparams : E.constructor_params)
              (mthds : F.fs string E.arrowT) (i : tags_t) :
     let extrn := {{{ Extern cparams { mthds } }}} in
-    ⦗ cs, fns, pgis, cis, pis, eis, errs ⦘
+    ⦗ cs, fns, pgis, cis, pis, eis, \Delta ⦘
       ⊢ extern e (cparams) { mthds } @ i
       ⊣ ⦗ eis, pis, cis, pgis, fns, e ↦ extrn;; cs ⦘ *)
-| chk_package (pkg : string) (cparams : E.constructor_params) (i : tags_t) :
+| chk_package (pkg : string)
+              (TS : list string)
+              (cparams : E.constructor_params) (i : tags_t) :
     let pkge := {{{ PackageType cparams }}} in
-    ⦗ cs, fns, pgis, cis, pis, eis, errs ⦘
-      ⊢ package pkg <[]> (cparams) @ i
+    ⦗ cs, fns, pgis, cis, pis, eis ⦘
+      ⊢ package pkg <TS> (cparams) @ i
       ⊣ ⦗ eis, pis, cis, pgis, fns, pkg ↦ pkge;; cs ⦘
 | chk_fruit_function (f : string) (params : E.params)
+                     (Δ : list string)
                      (τ : E.t) (body : ST.s tags_t) (i : tags_t)
-                     (Γ' Γ'' : gamma) (sg : signal) :
+                     (Γ' Γ'' : Gamma) (sg : signal) :
     bind_all params !{∅}! = Γ' ->
-    ⦃ fns, errs, Γ' ⦄ Function τ ⊢ body ⊣ ⦃ Γ'', sg ⦄ ->
+    ⦃ fns, Δ, Γ' ⦄ Function τ ⊢ body ⊣ ⦃ Γ'', sg ⦄ ->
     let func := P.Arrow params (Some τ) in
-    ⦗ cs, fns, pgis, cis, pis, eis, errs ⦘
-      ⊢ fn f <[]> (params) -> τ { body } @ i
+    ⦗ cs, fns, pgis, cis, pis, eis ⦘
+      ⊢ fn f <Δ> (params) -> τ { body } @ i
       ⊣ ⦗ eis, pis, cis, pgis, f ↦ func;;  fns, cs ⦘
-| chk_void_function (f : string) (params : E.params)
+| chk_void_function (f : string) (Δ : Delta)
+                    (params : E.params)
                     (body : ST.s tags_t) (i : tags_t)
-                    (Γ' Γ'' : gamma) (sg : signal) :
+                    (Γ' Γ'' : Gamma) (sg : signal) :
     bind_all params !{∅}! = Γ' ->
-    ⦃ fns, errs, Γ' ⦄ Void ⊢ body ⊣ ⦃ Γ'', sg ⦄ ->
+    ⦃ fns, Δ, Γ' ⦄ Void ⊢ body ⊣ ⦃ Γ'', sg ⦄ ->
     let func := P.Arrow params None in
-    ⦗ cs, fns, pgis, cis, pis, eis, errs ⦘
-      ⊢ void f <[]> (params) { body } @ i
+    ⦗ cs, fns, pgis, cis, pis, eis ⦘
+      ⊢ void f<Δ>(params) { body } @ i
       ⊣ ⦗ eis, pis, cis, pgis, f ↦ func;;  fns, cs ⦘
 | chk_topdecl_seq (d1 d2 : TD.d tags_t) (i : tags_t)
                   (eis' eis'' : eienv) (pgis' pgis'' : pkgienv)
                   (pis' pis'' : pienv) (cis' cis'' : cienv)
                   (fns' fns'' : fenv) (cs' cs'' : cenv) :
-    ⦗ cs, fns, pgis, cis, pis, eis, errs ⦘ ⊢ d1
+    ⦗ cs, fns, pgis, cis, pis, eis ⦘ ⊢ d1
     ⊣ ⦗ eis', pis', cis', pgis', fns', cs' ⦘ ->
-    ⦗ cs', fns', pgis', cis', pis', eis', errs ⦘ ⊢ d2
+    ⦗ cs', fns', pgis', cis', pis', eis' ⦘ ⊢ d2
     ⊣ ⦗ eis'', pis'', cis'', pgis'', fns'', cs'' ⦘ ->
-    ⦗ cs, fns, pgis, cis, pis, eis, errs ⦘ ⊢ d1 ;%; d2 @ i
+    ⦗ cs, fns, pgis, cis, pis, eis ⦘ ⊢ d1 ;%; d2 @ i
     ⊣ ⦗ eis'', pis'', cis'', pgis'', fns'', cs'' ⦘
 where
-"⦗ cs1 , fs1 , pgi1 , ci1 , pi1 , ei1 , ers ⦘ ⊢ d ⊣ ⦗ ei2 , pi2 , ci2 , pgi2 , fs2 , cs2 ⦘"
-  := (check_topdecl cs1 fs1 pgi1 ci1 pi1 ei1 ers d ei2 pi2 ci2 pgi2 fs2 cs2).
+"⦗ cs1 , fs1 , pgi1 , ci1 , pi1 , ei1 ⦘ ⊢ d ⊣ ⦗ ei2 , pi2 , ci2 , pgi2 , fs2 , cs2 ⦘"
+  := (check_topdecl cs1 fs1 pgi1 ci1 pi1 ei1 d ei2 pi2 ci2 pgi2 fs2 cs2).
 (**[]*)
