deps/poulet4/lib/P4cub/README.md
@@ -7,6 +7,7 @@
 - `P4cub/Static`: Static semantics, including typechecking.
 
 - `P4cub/Architecture`: The representation of packets, targets, externs, & pipeline.
+**UPDATE**: will be repaced entirely by `p4light`'s `Target.v` via translations to and from requisite data types.
 
 - `P4cub/BigStep`: Big-step evaluation semantics.
 
@@ -17,16 +18,13 @@
 - `Envn.v`: Generic notion of environments for `p4cub` semantics.
 
 - `Metamorphosis.v`: Translation from "simplified" `p4light` syntax to `p4cub`.
+**UPDATE**: This will be replaced by another translation defined in branch `ec-vcgen`.
 
 - `README.md`: This file :).
 
 ### Updates:
 
-- The entire `P4cub` directory is being restructured as its codebase expands.
-
-- An experimental representation of target architectures, `P4cub/Architecture.v` is now used in the big-step semantics. It is primarily used to dispatch `extern` method calls.
-
-- Packets now exist in `p4cub` & are threaded through the big-step semantics.
+- Type variables & specialization are now supported in `p4cub`.
 
 ### Goals:
 
@@ -42,8 +40,16 @@
 
 ### TODOs:
 
+- `p4cub` Notations are messy and need to be edited and refactored
+
+- Many results in `p4cub` have become invalidated by the introduction of type variables.
+This should not pose too large of a problem to resolve.
+
+- Use of induction within induction needs to stop in `p4cub` proofs.
+
 - The core codebase for `p4cub` packets/target/architecture representaion should exist within one directory.
 
 - Constructor parameters currently do nothing for externs. Maybe `p4cub` externs need not have them?
 
 - Explore common ground between `p4light` & `p4cub` architecture/target/packet models.
+**UPDATE**: `p4cub` will use `p4light`'s `Target.v` with translations between the requisite data types.
